Moved Coq examples to their own file.

theory/CoreRel/Embed.v
@@ -114,11 +114,11 @@ Section Embed.
     forall st1 st2 a,
       aeval st1 a = aeval (M := (@prod_M M)) (st1, st2) (inj_id_aexp_l a).
   Proof.
- 
+
     induction a; simpl; eauto.
   Qed.
 
- 
+
 
   Lemma inj_id_aexp_r_aeval :
     forall st1 st2 a,
@@ -131,7 +131,7 @@ Section Embed.
     forall st1 st2 b,
       beval st1 b = beval (M := (@prod_M M)) (st1, st2) (inj_id_bexp_l b).
   Proof.
-  
+
     induction b; simpl; eauto;
       try erewrite !inj_id_aexp_l_aeval;
       rewrite ?IHb;
@@ -237,7 +237,7 @@ Section Embed.
     - specialize (E_Ass (st, st2) (inj_id_aexp_l a) n (inl x));
         simpl; intro H0; apply H0.
       rewrite <- inj_id_aexp_l_aeval; assumption.
-    - 
+    -
     econstructor;
         try rewrite <- inj_id_bexp_l_beval; eauto.
     - eapply E_IfFalse;
@@ -488,18 +488,13 @@ Compute reify_com <{ <| CSkip | CSkip |> }>.
 
 End Embed.
 
-Section rel_verification.
 From CR Require Import Hoare.
+
+Section rel_verification.
     Definition I := @prod_I string.
     Context {M : Type -> Type}.
     Context {id : Id string M}.
 
-  
-  (*Definition Assertion := CR.Hoare.Definitions.Assertion. *)
-  (*Import CR.Hoare.Definitions.*)
-   Set Printing All.
-   
-   
   Definition hoare_triple_product
              (P : Assertion) (r : @com I ) (Q : Assertion) : Prop := hoare_triple P r Q.
     (*forall st1 st2 st1' st2',
@@ -512,7 +507,6 @@ From CR Require Import Hoare.
     forall st1 st2 st1' st2',
       P (st1 ,st2)  ->
       ceval s1 st1 st1' ->
-      (*st1 =[s1]=> st1' ->*)
       ceval s2 st2 st2' ->
       Q (st1', st2').
 
@@ -540,168 +534,7 @@ From CR Require Import Hoare.
     intros; eexists; split; try reflexivity; intros.
     eapply reify_is_iso in H1.
     unfold embed_com in H1; inversion H1; subst. destruct st.
-    eapply H; eassumption. 
+    eapply H; eassumption.
   Qed.
 
 End rel_verification.
-
-Module Proofs.
-
-  Import Imp.Syntax.notations.
-  Import Imp.Semantics.notations.
-  Import CR.Syntax.notations.
-  Import CR.Semantics.notations.
-  Import Coq.Setoids.Setoid.
-  Import CR.Hoare.
-
-  Definition I := string.
-  Context {M : Type -> Type}.
-  Context {id : Id I M}.
-
-  Variable W X Y Z : I.
-
-  Lemma comm_def : forall c1 c2 c3 c4,
-      align_eqv <{ <|c1; c2 | c3; c4|> }> <{ <| c1 | c3|> ;; <| c2 | c4 |> }>.
-  Proof.
-    intros. rewrite rel_def. rewrite  prod_hom_l. rewrite prod_hom_r.
-    rewrite prod_seq_assoc.
-    rewrite <- prod_seq_assoc with (r3 := <{<| skip | c4 |>}>) . rewrite <- rel_comm.
-    rewrite <- !prod_seq_assoc.  rewrite <- rel_def.
-    rewrite prod_seq_assoc. rewrite <- rel_def. reflexivity.
-  Qed.
-
-  Lemma comm_skip : forall c1 c3 c4,
-      align_eqv <{ <|c1 | c3; c4|> }> <{ <| c1 | c3|> ;; <| skip | c4 |> }>.
-  Proof.
-    intros. rewrite rel_def. rewrite prod_hom_r. rewrite <- prod_seq_assoc.
-    rewrite <- rel_def. reflexivity.
-  Qed.
-
-
- Definition ex_1 Y Z : @algn_com I :=
-  <{
-     <| Y := 0 | Y := 0 |>;;
-     <| Z :=  2 * 2 | Z := 2 * 2|> }>.
-
- Compute reify_com (ex_1 Y Z).
-
-
- Definition ex_2 Y Z : @algn_com I :=
-   <{ <| Y := 0 ; Z := 2 * 2 | skip |>;;
-      <| skip | Y :=  0 ; Z := 2 * 2|> }>.
-
-
- Compute reify_com (ex_2 Y Z).
-
- Lemma example_12 : align_eqv  (ex_1 Y Z) (ex_2 Y Z).
- Proof.
-   unfold ex_2. rewrite <- rel_def.  rewrite comm_def. reflexivity.
- Qed.
-
- Definition AId' : I -> aexp := AId.
- Coercion AId' : I >-> aexp.
-
- Definition kestrel_paper_p1 : @com I :=
-   <{Y := 0;
-     Z := 2 * X;
-     while (~(Z <= 0)) do
-       Z := Z - 1;
-       Y := Y + X;
-       Z := Z - 1;
-       Y := Y + X
-       end}>.
-
-  Definition kestrel_paper_p2 : @com I :=
-    <{ Y := 0;
-      Z := X;
-     while ~ (Z <= 0) do
-       Z := Z - 1;
-       Y := Y + X
-     end; Y := Y * 2 }>.
-
- Definition kestrel_paper_example_1_prod_efficient : @algn_com I :=
- <{ <| Y := 0 | Y := 0 |>;;
-     <| Z :=  2 * X | Z := X|>;;
-   (whileR <| ~(Z <= 0) | ~(Z <= 0) |> do
-            <| Z := Z - 1; Y := Y + X;
-               Z :=  Z - 1; Y := Y + X |
-               Z :=  Z - 1; Y := Y + X |> end;; <|while  ~(Z <= 0) do Z := Z - 1; Y := Y + X;
-               Z :=  Z - 1; Y := Y + X end | while ~(Z <= 0) do  Z :=  Z - 1; Y := Y + X end|>);;
-     <| skip | Y := Y * 2 |> }>.
-
-  Definition kestrel_paper_skip1 : @com I := <{skip}>.
-
-  Definition kestrel_paper_skip2 : @com I := <{ skip }>.
-
-  Definition kestrel_paper_skip_prod_efficient : @algn_com I :=
- <{ <|skip | skip|>}>.
-
-  Definition kestrel_paper_while1 : @com I := <{while false do skip end}>.
-
-  Definition kestrel_paper_while2 : @com I := <{while false do skip end}>.
-  
-  Definition kestrel_paper_while_prod_efficient : @algn_com I :=
- <{ whileR <| false | false |> do <|skip | skip|> end ;; 
-    <| while false do skip end | while false do skip end |>}>.  
-
-
- Lemma paper_example1_eqv : align_eqv (embed_com kestrel_paper_p1 kestrel_paper_p2)
-                                  kestrel_paper_example_1_prod_efficient.
- Proof.
-   unfold kestrel_paper_p1, kestrel_paper_p2; unfold embed_com; simpl.
-   rewrite comm_def.
-   rewrite comm_def.
-   rewrite comm_skip.
-   rewrite whileR_lockstep.
-   reflexivity.
- Qed.
-
- Lemma paper_while_eqv : align_eqv (embed_com kestrel_paper_while1 kestrel_paper_while2)
-                                  kestrel_paper_while_prod_efficient.
- Proof.
-  unfold kestrel_paper_while1, kestrel_paper_while2; unfold embed_com; simpl. 
-  rewrite whileR_lockstep. unfold kestrel_paper_while_prod_efficient. reflexivity.
- Qed.
-
-
- Lemma paper_skip_eqv : align_eqv (embed_com kestrel_paper_skip1 kestrel_paper_skip2)
-                                  kestrel_paper_skip_prod_efficient.
- Proof.
-   unfold kestrel_paper_skip1, kestrel_paper_skip2; unfold embed_com; simpl.
-   unfold kestrel_paper_skip_prod_efficient. reflexivity.
- Qed.
-
- Definition equiv_state : @Assertion M :=
-   fun st: state => forall id : I, (st : @prod_M M nat) !!! (@inl I I id : prod_I) = (st : @prod_M M nat) !!! (@inr I I id : prod_I).
-
-
-  Ltac assn_auto :=
-  try auto; 
-  try (unfold assert_implies, assn_sub, insert;
-       intros; simpl in *; lia).
-
- Lemma paper_skip :
-   hoare_triple_relational equiv_state
-                           kestrel_paper_skip1 kestrel_paper_skip2
-                           equiv_state.
- Proof.
-  eapply hoare_triple_prod_a. split.
-  symmetry. exact paper_skip_eqv.
-  simpl. unfold hoare_triple_product, equiv_state. 
-  eapply hoare_seq. apply hoare_skip. apply hoare_skip. 
- Qed.
-
-
- Lemma paper_example1 :
-   hoare_triple_relational equiv_state
-                           kestrel_paper_p1 kestrel_paper_p2
-                           equiv_state.
- Proof.
-   eapply hoare_triple_prod_a.
-   split.
-   - symmetry; exact paper_example1_eqv.
-   - simpl. unfold hoare_triple_product, equiv_state. intros.
-     eapply hoare_seq. eapply hoare_seq. eapply hoare_while.
- Admitted.
-
-End Proofs.
