theory/CoreRel/Examples.v
@@ -1,0 +1,149 @@
+From Coq Require Import Strings.String.
+From Coq Require Import Setoids.Setoid.
+From Common Require Import Id Fixpoints.
+From Imp Require Import Syntax Semantics.
+From CR Require Import Syntax Semantics Hoare Equiv Embed.
+
+Import Imp.Syntax.notations.
+Import Imp.Semantics.notations.
+Import CR.Syntax.notations.
+Import CR.Semantics.notations.
+Import CR.Semantics.notations.
+
+Definition I := string.
+Context {M : Type -> Type}.
+Context {id : Id I M}.
+
+Section Examples.
+
+  Variable W X Y Z : I.
+
+  Lemma comm_def : forall c1 c2 c3 c4,
+      align_eqv <{ <|c1; c2 | c3; c4|> }> <{ <| c1 | c3|> ;; <| c2 | c4 |> }>.
+  Proof.
+    intros. rewrite rel_def. rewrite  prod_hom_l. rewrite prod_hom_r.
+    rewrite prod_seq_assoc.
+    rewrite <- prod_seq_assoc with (r3 := <{<| skip | c4 |>}>) . rewrite <- rel_comm.
+    rewrite <- !prod_seq_assoc.  rewrite <- rel_def.
+    rewrite prod_seq_assoc. rewrite <- rel_def. reflexivity.
+  Qed.
+
+  Lemma comm_skip : forall c1 c3 c4,
+      align_eqv <{ <|c1 | c3; c4|> }> <{ <| c1 | c3|> ;; <| skip | c4 |> }>.
+  Proof.
+    intros. rewrite rel_def. rewrite prod_hom_r. rewrite <- prod_seq_assoc.
+    rewrite <- rel_def. reflexivity.
+  Qed.
+
+  Definition ex_1 Y Z : @algn_com I :=
+    <{
+     <| Y := 0 | Y := 0 |>;;
+     <| Z :=  2 * 2 | Z := 2 * 2|> }>.
+
+  Compute reify_com (ex_1 Y Z).
+
+  Definition ex_2 Y Z : @algn_com I :=
+   <{ <| Y := 0 ; Z := 2 * 2 | skip |>;;
+      <| skip | Y :=  0 ; Z := 2 * 2|> }>.
+
+  Compute reify_com (ex_2 Y Z).
+
+  Lemma example_12 : align_eqv  (ex_1 Y Z) (ex_2 Y Z).
+  Proof.
+    unfold ex_2. rewrite <- rel_def.  rewrite comm_def. reflexivity.
+  Qed.
+
+  Definition AId' : I -> aexp := AId.
+  Coercion AId' : I >-> aexp.
+
+  Definition kestrel_paper_p1 : @com I :=
+   <{Y := 0;
+     Z := 2 * X;
+     while (~(Z <= 0)) do
+       Z := Z - 1;
+       Y := Y + X;
+       Z := Z - 1;
+       Y := Y + X
+       end}>.
+
+  Definition kestrel_paper_p2 : @com I :=
+    <{ Y := 0;
+      Z := X;
+     while ~ (Z <= 0) do
+       Z := Z - 1;
+       Y := Y + X
+     end; Y := Y * 2 }>.
+
+  Definition kestrel_paper_example_1_prod_efficient : @algn_com I :=
+ <{ <| Y := 0 | Y := 0 |>;;
+     <| Z :=  2 * X | Z := X|>;;
+   (whileR <| ~(Z <= 0) | ~(Z <= 0) |> do
+            <| Z := Z - 1; Y := Y + X;
+               Z :=  Z - 1; Y := Y + X |
+               Z :=  Z - 1; Y := Y + X |> end;; <|while  ~(Z <= 0) do Z := Z - 1; Y := Y + X;
+               Z :=  Z - 1; Y := Y + X end | while ~(Z <= 0) do  Z :=  Z - 1; Y := Y + X end|>);;
+     <| skip | Y := Y * 2 |> }>.
+
+  Definition kestrel_paper_skip1 : @com I := <{skip}>.
+
+  Definition kestrel_paper_skip2 : @com I := <{ skip }>.
+
+  Definition kestrel_paper_skip_prod_efficient : @algn_com I :=
+    <{ <|skip | skip|>}>.
+
+  Definition kestrel_paper_while1 : @com I := <{while false do skip end}>.
+
+  Definition kestrel_paper_while2 : @com I := <{while false do skip end}>.
+
+  Definition kestrel_paper_while_prod_efficient : @algn_com I :=
+    <{ whileR <| false | false |> do <|skip | skip|> end ;;
+    <| while false do skip end | while false do skip end |>}>.
+
+
+  Lemma paper_example1_eqv : align_eqv (embed_com kestrel_paper_p1 kestrel_paper_p2)
+                                       kestrel_paper_example_1_prod_efficient.
+  Proof.
+    unfold kestrel_paper_p1, kestrel_paper_p2; unfold embed_com; simpl.
+    rewrite comm_def.
+    rewrite comm_def.
+    rewrite comm_skip.
+    rewrite whileR_lockstep.
+    reflexivity.
+  Qed.
+
+  Lemma paper_while_eqv : align_eqv (embed_com kestrel_paper_while1 kestrel_paper_while2)
+                                    kestrel_paper_while_prod_efficient.
+  Proof.
+    unfold kestrel_paper_while1, kestrel_paper_while2; unfold embed_com; simpl.
+    rewrite whileR_lockstep. unfold kestrel_paper_while_prod_efficient. reflexivity.
+  Qed.
+
+
+  Lemma paper_skip_eqv : align_eqv (embed_com kestrel_paper_skip1 kestrel_paper_skip2)
+                                   kestrel_paper_skip_prod_efficient.
+  Proof.
+    unfold kestrel_paper_skip1, kestrel_paper_skip2; unfold embed_com; simpl.
+    unfold kestrel_paper_skip_prod_efficient. reflexivity.
+  Qed.
+
+  Definition equiv_state : @Assertion M :=
+    fun st: state => forall id : I, (st : @prod_M M nat) !!! (@inl I I id : prod_I) = (st : @prod_M M nat) !!! (@inr I I id : prod_I).
+
+
+  Ltac assn_auto :=
+    try auto;
+    try (unfold assert_implies, assn_sub, insert;
+         intros; simpl in *; lia).
+
+  Lemma paper_skip :
+    hoare_triple_relational equiv_state
+                            kestrel_paper_skip1 kestrel_paper_skip2
+                            equiv_state.
+  Proof.
+    eapply hoare_triple_prod_a. split.
+    symmetry. exact paper_skip_eqv.
+    simpl. unfold hoare_triple_product, equiv_state.
+    eapply hoare_seq. apply hoare_skip. apply hoare_skip.
+  Qed.
+
+End Examples.
